\documentclass[11pt]{article}
\usepackage{xeCJK}
\usepackage{changepage}
\usepackage{bussproofs}
\usepackage[top=2cm,left=0.5cm,right=0.5cm,bottom=2cm]{geometry}

\title{HW1}
\author{r08725027 林宏陽}
\date{\today}

\begin{document}
	\maketitle
	\begin{enumerate}
	\item
		\begin{enumerate}
		\item Because both CNF and DNF must be NNF, we apply the Double Negation law, De Morgan's law and the following equivalences to every occurrence in the target formula recursively.
			$$ \phi \to \psi \equiv \neg \phi \lor \psi $$
			$$ \phi \leftrightarrow \psi \equiv (\phi \to \psi) \land (\psi \to \phi) $$
		\item For every subformula in the form $\phi \lor (\psi_{1} \land \psi_{2})$, substitute it by $(\phi \lor \psi_{1}) \land (\phi \lor \psi_{2})$ by using the distributivity law recursively. Similarly, for every subformula in the form $(\phi_{1} \land \phi_{2}) \lor \psi$, substitute it by $(\phi_{1} \lor \psi) \land (\phi_{2} \lor \psi)$. 
		\end{enumerate}

		After step (b), there is no such two forms in the target formula, therefore, it is transformed into the formula in CNF.
		For the case of DNF, simply dualise step (b). (swap $\land$ and $\lor$)
		
	\item 
		\begin{enumerate}
			\item ~
			\begin{prooftree}
				\AxiomC{}
				\RightLabel{$(Ax)$}
				\UnaryInfC{$p \lor q \to r, p \vdash p \lor q \to r$}

				\AxiomC{}
				\RightLabel{$(Ax)$}
				\UnaryInfC{$p \lor q \to r, p \vdash p$}
				\RightLabel{$(\lor I_{1})$}
				\UnaryInfC{$p \lor q \to r, p \vdash p \lor q$}

				\RightLabel{$(\to E)$}
				\BinaryInfC{$p \lor q \to r, p \vdash r$}
				\RightLabel{$(\to I)$}
				\UnaryInfC{$p \lor q \to r \vdash p \to r$}

				\AxiomC{$\alpha$}
				\RightLabel{$(\to I)$}
				\UnaryInfC{$p \lor q \to r \vdash q \to r$}
				\RightLabel{$(\land I)$}
				\BinaryInfC{$p \lor q \to r \vdash (p \to r) \land (q \to r)$}
			\end{prooftree}
			where $\alpha$ is the following tree :
			\begin{prooftree}
				\AxiomC{}
				\RightLabel{$(Ax)$}
				\UnaryInfC{$p \lor q \to r, q \vdash p \lor q \to r$}

				\AxiomC{}
				\RightLabel{$(Ax)$}
				\UnaryInfC{$p \lor q \to r, q \vdash q$}
				\RightLabel{$(\lor I_{2})$}
				\UnaryInfC{$p \lor q \to r, q \vdash p \lor q$}
				\RightLabel{$(\to E)$}
				\BinaryInfC{$p \lor q \to r, q \vdash r$}
			\end{prooftree}
		
			\item ~
			\begin{prooftree}
				\AxiomC{}
				\RightLabel{$(Ax)$}
				\UnaryInfC{$p \land q \to r, p, q \vdash p \land q \to r$}

				\AxiomC{}
				\RightLabel{$(Ax)$}
				\UnaryInfC{$p \land q \to r, p, q \vdash p$}

				\AxiomC{}
				\RightLabel{$(Ax)$}
				\UnaryInfC{$p \land q \to r, p, q \vdash q$}

				\RightLabel{$(\land I)$}
				\BinaryInfC{$p \land q \to r, p, q \vdash p \land q$}

				\RightLabel{$(\to E)$}
				\BinaryInfC{$p \land q \to r, p, q \vdash r$}
				\RightLabel{$(\to I)$}
				\UnaryInfC{$p \land q \to r, p \vdash q \to r$}
				\RightLabel{$(\to I)$}
				\UnaryInfC{$p \land q \to r \vdash p \to (q \to r)$}
				\RightLabel{$(\to I)$}
				\UnaryInfC{$\vdash (p \land q \to r) \to (p \to (q \to r))$}
			\end{prooftree}
		\end{enumerate}
	\newpage
	\item 
		\begin{enumerate}
			\item ~
			\begin{prooftree}
				\AxiomC{}
				\RightLabel{$(Ax)$}
				\UnaryInfC{$\neg p \lor q, p \vdash \neg p \lor q$}

				\AxiomC{}
				\RightLabel{$(Ax)$}
				\UnaryInfC{$\neg p \lor q, p, \neg p, \neg q \vdash p$}
				\AxiomC{}
				\RightLabel{$(Ax)$}
				\UnaryInfC{$\neg p \lor q, p, \neg p, \neg q \vdash \neg p$}
				\RightLabel{$(\land I)$}
				\BinaryInfC{$\neg p \lor q, p, \neg p, \neg q \vdash p \land \neg p$}
				\RightLabel{$(\neg I)$}
				\UnaryInfC{$\neg p \lor q, p, \neg p \vdash \neg \neg q$}
				\RightLabel{$(\neg \neg E)$}
				\UnaryInfC{$\neg p \lor q, p, \neg p \vdash q$}

				\AxiomC{}
				\RightLabel{$(Ax)$}
				\UnaryInfC{$\neg p \lor q, p, q \vdash q$}

				\RightLabel{$(\lor E)$}
				\TrinaryInfC{$\neg p \lor q, p \vdash q$}
				\RightLabel{$(\to I)$}
				\UnaryInfC{$\neg p \lor q \vdash p \to q$}
				\RightLabel{$(\to I)$}
				\UnaryInfC{$\vdash (\neg p \lor q) \to (p \to q)$}
			\end{prooftree}

			\item ~
			\begin{prooftree}
				\AxiomC{$\beta$}

				\AxiomC{}
				\RightLabel{$(Ax)$}
				\UnaryInfC{$(p \to q) \to p, \neg p \vdash \neg p$}

				\RightLabel{$(\land I)$}
				\BinaryInfC{$(p \to q) \to p, \neg p \vdash p \land \neg p$}
				\RightLabel{$(\neg I)$}
				\UnaryInfC{$(p \to q) \to p \vdash \neg \neg p$}
				\RightLabel{$(\neg \neg E)$}
				\UnaryInfC{$(p \to q) \to p \vdash p$}
				\RightLabel{$(\to I)$}
				\UnaryInfC{$\vdash ((p \to q) \to p) \to p$}
			\end{prooftree}
			where $\beta$ is the following tree :
			\begin{prooftree}
				\AxiomC{}
				\RightLabel{$(Ax)$}
				\UnaryInfC{$(p \to q) \to p, \neg p \vdash (p \to q) \to p$}

				\AxiomC{}
				\RightLabel{$(Ax)$}
				\UnaryInfC{$(p \to q) \to p, \neg p, p, \neg q \vdash p$}
				\AxiomC{}
				\RightLabel{$(Ax)$}
				\UnaryInfC{$(p \to q) \to p, \neg p, p, \neg q \vdash \neg p$}
				\RightLabel{$(\land I)$}
				\BinaryInfC{$(p \to q) \to p, \neg p, p, \neg q \vdash p \land \neg p$}
				\RightLabel{$(\neg I)$}
				\UnaryInfC{$(p \to q) \to p, \neg p, p \vdash \neg \neg q$}
				\RightLabel{$(\neg \neg E)$}
				\UnaryInfC{$(p \to q) \to p, \neg p, p \vdash q$}
				\RightLabel{$(\to I)$}
				\UnaryInfC{$(p \to q) \to p, \neg p \vdash p \to q$}

				\RightLabel{$(\to E)$}
				\BinaryInfC{$(p \to q) \to p, \neg p \vdash p$}
			\end{prooftree}

		\end{enumerate}
	\end{enumerate}
\end{document}