\documentclass[10pt]{article}
\usepackage{xeCJK}
\usepackage{changepage}
\usepackage{bussproofs}
\usepackage[top=2cm,left=0.25cm,right=0.25cm,bottom=2cm]{geometry}

\title{HW2}
\author{r08725027 林宏陽}
\date{\today}

\begin{document}
	\maketitle
	\begin{enumerate}
	\item 
		\begin{enumerate}
			\item ~
			\begin{prooftree}
				\AxiomC{}
				\RightLabel{$(Ax)$}
				\UnaryInfC{$\forall x (P(x) \to Q (x)), \forall x P(x) \vdash \forall x (P(x) \to Q (x))$}
				\RightLabel{$(\forall E)$}
				\UnaryInfC{$\forall x (P(x) \to Q (x)), \forall x P(x) \vdash P(y) \to Q(y)$}

				\AxiomC{}
				\RightLabel{$(Ax)$}
				\UnaryInfC{$\forall x (P(x) \to Q (x)), \forall x P(x) \vdash \forall x P(x)$}
				\RightLabel{$(\forall E)$}
				\UnaryInfC{$\forall x (P(x) \to Q (x)), \forall x P(x) \vdash P(y)$}

				\RightLabel{$(\to E)$}
				\BinaryInfC{$\forall x (P(x) \to Q (x)), \forall x P(x) \vdash Q(y)$}
				\RightLabel{$(\forall I)$}
				\UnaryInfC{$\forall x (P(x) \to Q (x)), \forall x P(x) \vdash \forall x Q(x)$}
				\RightLabel{$(\to I)$}
				\UnaryInfC{$\forall x (P(x) \to Q (x)) \vdash \forall x P(x) \to \forall x Q(x)$}
			\end{prooftree}
			\item ~
			\begin{prooftree}
				\AxiomC{}
				\RightLabel{$(Ax)$}
				\UnaryInfC{$\exists x \forall y P(x,y) \vdash \exists x \forall y P(x,y)$}

				\AxiomC{}
				\RightLabel{$(Ax)$}
				\UnaryInfC{$\exists x \forall y P(x,y), \forall y P(w,y) \vdash \forall y P(w,y)$}

				\RightLabel{$(\exists E)$}
				\BinaryInfC{$\exists x \forall y P(x,y) \vdash \forall y P(w,y)$}
				\RightLabel{$(\forall E)$}
				\UnaryInfC{$\exists x \forall y P(x,y) \vdash P(w,z)$}
				\RightLabel{$(\exists I)$}
				\UnaryInfC{$\exists x \forall y P(x,y) \vdash \exists x P(x,z)$}
				\RightLabel{$(\forall I)$}
				\UnaryInfC{$\exists x \forall y P(x,y) \vdash \forall y \exists x P(x,y)$}

				\RightLabel{$(\to I)$}
				\UnaryInfC{$\vdash \exists x \forall y P(x,y) \to \forall y \exists x P(x,y)$}
			\end{prooftree}
			\item ~
			\begin{prooftree}
				\AxiomC{}
				\RightLabel{$(Ax)$}
				\UnaryInfC{$\forall x (A(x) \to B), \exists x A(x), A(y) \vdash \forall x (A(x) \to B)$}
				\RightLabel{$(\forall E)$}
				\UnaryInfC{$\forall x (A(x) \to B), \exists x A(x), A(y) \vdash A(y) \to B$}

				\AxiomC{$\alpha$}

				\RightLabel{$(\to E)$}
				\BinaryInfC{$\forall x (A(x) \to B), \exists x A(x) \vdash B$}
				\RightLabel{$(\to I)$}
				\UnaryInfC{$\forall x (A(x) \to B) \vdash \exists x A(x) \to B$}
			\end{prooftree}
			where $\alpha$ is the following tree :
			\begin{prooftree}
				\AxiomC{}
				\RightLabel{$(Ax)$}
				\UnaryInfC{$\forall x (A(x) \to B), \exists x A(x), A(y) \vdash \exists x A(x)$}

				\AxiomC{}
				\RightLabel{$(Ax)$}
				\UnaryInfC{$\forall x (A(x) \to B), \exists x A(x), A(y) \vdash A(y)$}

				\RightLabel{$(\exists E)$}
				\BinaryInfC{$\forall x (A(x) \to B), \exists x A(x) \vdash A(y)$}
			\end{prooftree}
		\end{enumerate}
	
	\item 
		\begin{enumerate}
			\item ~
			\begin{prooftree}
				\AxiomC{}
				\RightLabel{$(Ax)$}
				\UnaryInfC{$t_{2} = t_{1} \vdash t_{2} = t_{1}$}

				\AxiomC{}
				\RightLabel{$(=I)$}
				\UnaryInfC{$t_{2} = t_{1} \vdash t_{2} = t_{2}$}

				\RightLabel{$(=E)$}
				\BinaryInfC{$t_{2} = t_{1} \vdash t_{1} = t_{2}$}
			\end{prooftree}

			\item ~
			\begin{prooftree}
				\AxiomC{}
				\RightLabel{$(Ax)$}
				\UnaryInfC{$t_{1} = t_{2}, t_{2} = t_{3} \vdash t_{2} = t_{3}$}

				\AxiomC{}
				\RightLabel{$(Ax)$}
				\UnaryInfC{$t_{1} = t_{2}, t_{2} = t_{3} \vdash t_{1} = t_{2}$}

				\RightLabel{$(=E)$}
				\BinaryInfC{$t_{1} = t_{2}, t_{2} = t_{3} \vdash t_{1} = t_{3}$}
			\end{prooftree}
		\end{enumerate}
	
	\item 
		\begin{enumerate}
			\item ~
			\begin{prooftree}
				\AxiomC{}
				\RightLabel{$(Ax)$}
				\UnaryInfC{$\Gamma, t_{2} = t_{1} \vdash t_{1} = t_{2}$}
				\RightLabel{$(\to I)$}
				\UnaryInfC{$\Gamma \vdash (t_{2} = t_{1}) \to (t_{1} = t_{2})$}

				\AxiomC{}
				\RightLabel{$(Ax)$}
				\UnaryInfC{$\Gamma \vdash t_{2} = t_{1}$}

				\RightLabel{$(\to E)$}
				\BinaryInfC{$\Gamma \vdash t_{1} = t_{2}$}
			\end{prooftree}

			\item ~
			\begin{prooftree}
				\AxiomC{}
				\RightLabel{$(Ax)$}
				\UnaryInfC{$\Gamma, t_{1} = t_{2}, t_{2} = t_{3} \vdash t_{1} = t_{3}$}
				\RightLabel{$(\to I)$}
				\UnaryInfC{$\Gamma, t_{1} = t_{2} \vdash (t_{2} = t_{3}) \to (t_{1} = t_{3})$}
				\RightLabel{$(\to I)$}
				\UnaryInfC{$\Gamma \vdash (t_{1} = t_{2}) \to ((t_{2} = t_{3}) \to (t_{1} = t_{3}))$}

				\AxiomC{}
				\RightLabel{$(Ax)$}
				\UnaryInfC{$\Gamma \vdash t_{1} = t_{2}$}

				\RightLabel{$(\to E)$}
				\BinaryInfC{$\Gamma \vdash (t_{2} = t_{3}) \to (t_{1} = t_{3})$}

				\AxiomC{}
				\RightLabel{$(Ax)$}
				\UnaryInfC{$\Gamma \vdash t_{2} = t_{3}$}

				\RightLabel{$(\to E)$}
				\BinaryInfC{$\Gamma \vdash t_{1} = t_{3}$}
			\end{prooftree}
		\end{enumerate}
		\item 
		\begin{enumerate}
			\item ~
			Let $\Gamma$ denote $M, x \cdot y = x \cdot z$.
			\begin{prooftree}
				\AxiomC{}
				\RightLabel{$(Ax)$}
				\UnaryInfC{$\Gamma \vdash \forall a ((a \cdot e = a) \land (e \cdot a = a))$}
				\RightLabel{$(\forall E)$}
				\UnaryInfC{$\Gamma \vdash (z \cdot e = z) \land (e \cdot z = z)$}
				\RightLabel{$(\land E_{2})$}
				\UnaryInfC{$\Gamma \vdash e \cdot z = z$}

				\AxiomC{}
				\RightLabel{$(Ax)$}
				\UnaryInfC{$\Gamma \vdash \forall a ((e = a^{-1} \cdot a) \land (a^{-1} \cdot a = e))$}
				\RightLabel{$(\forall E)$}
				\UnaryInfC{$\Gamma \vdash (e = x^{-1} \cdot x) \land (x^{-1} \cdot x = e)$}
				\RightLabel{$(\land E_{2})$}
				\UnaryInfC{$\Gamma \vdash x^{-1} \cdot x = e$}

				\AxiomC{$\alpha$}

				\RightLabel{$(= E)$}
				\BinaryInfC{$\Gamma \vdash y = e \cdot z$}

				\RightLabel{$(= E)$}
				\BinaryInfC{$\Gamma \vdash y = z$}
				\RightLabel{$(\to I)$}
				\UnaryInfC{$M \vdash (x \cdot y = x \cdot z) \to y = z$}
				\RightLabel{$(\forall I)$}
				\UnaryInfC{$M \vdash \forall c ((x \cdot y = x \cdot c) \to y = c)$}
				\RightLabel{$(\forall I)$}
				\UnaryInfC{$M \vdash \forall b \forall c ((x \cdot b = x \cdot c) \to b = c)$}
				\RightLabel{$(\forall I)$}
				\UnaryInfC{$M \vdash \forall a \forall b \forall c ((a \cdot b = a \cdot c) \to b = c)$}
			\end{prooftree}
			where $\alpha$ is the following tree :
			\begin{prooftree}
				\AxiomC{}
				\RightLabel{$(Ax)$}
				\UnaryInfC{$\Gamma \vdash \forall a \forall b \forall c (a \cdot (b \cdot c) = (a \cdot b) \cdot c)$}
				\RightLabel{$(\forall E)$}
				\UnaryInfC{$\Gamma \vdash \forall b \forall c (x^{-1} \cdot (b \cdot c) = (x^{-1} \cdot b) \cdot c)$}
				\RightLabel{$(\forall E)$}
				\UnaryInfC{$\Gamma \vdash \forall c (x^{-1} \cdot (x \cdot c) = (x^{-1} \cdot x) \cdot c)$}
				\RightLabel{$(\forall E)$}
				\UnaryInfC{$\Gamma \vdash x^{-1} \cdot (x \cdot z) = (x^{-1} \cdot x) \cdot z$}

				\AxiomC{}
				\UnaryInfC{$\Gamma \vdash x \cdot y = x \cdot z$}

				\AxiomC{$\beta$}

				\RightLabel{$(=E)$}
				\BinaryInfC{$\Gamma \vdash y = x^{-1} \cdot (x \cdot z)$}

				\RightLabel{$(=E)$}
				\BinaryInfC{$\Gamma \vdash y = (x^{-1} \cdot x) \cdot z$}
			\end{prooftree}
			$\beta$ :
			\begin{prooftree}
				\AxiomC{}
				\RightLabel{$(Ax)$}
				\UnaryInfC{$\Gamma \vdash \forall b \forall c ((a \cdot b) \cdot c = a \cdot (b \cdot c))$}
				\RightLabel{$(\forall E)$}
				\UnaryInfC{$\Gamma \vdash \forall b \forall c ((x^{-1} \cdot b) \cdot c = x^{-1} \cdot (b \cdot c))$}
				\RightLabel{$(\forall E)$}
				\UnaryInfC{$\Gamma \vdash \forall c ((x^{-1} \cdot x) \cdot c = x^{-1} \cdot (x \cdot c))$}
				\RightLabel{$(=E)$}
				\UnaryInfC{$\Gamma \vdash (x^{-1} \cdot x) \cdot y = x^{-1} \cdot (x \cdot y)$}

				\AxiomC{}
				\RightLabel{$(Ax)$}
				\UnaryInfC{$\Gamma \vdash \forall a ((a^{-1} \cdot a = e) \land (e = a^{-1} \cdot a))$}
				\RightLabel{$(\forall E)$}
				\UnaryInfC{$\Gamma \vdash (x^{-1} \cdot x = e) \land (e = x^{-1} \cdot x)$}
				\RightLabel{$(\land E_{2})$}
				\UnaryInfC{$\Gamma \vdash e = x^{-1} \cdot x$}

				\AxiomC{$\gamma$}

				\RightLabel{$(=E)$}
				\BinaryInfC{$\Gamma \vdash y = (x^{-1} \cdot x) \cdot y$}

				\RightLabel{$(=E)$}
				\BinaryInfC{$\Gamma \vdash y = x^{-1} \cdot (x \cdot y)$}
			\end{prooftree}
			$\gamma$ :
			\begin{prooftree}
				\AxiomC{}
				\RightLabel{$(Ax)$}
				\UnaryInfC{$\Gamma \vdash \forall a ((a \cdot e = a) \land (e \cdot a = a))$}
				\RightLabel{$(\forall E)$}
				\UnaryInfC{$\Gamma \vdash (y \cdot e = y) \land (e \cdot y = y)$}
				\RightLabel{$(\land E_{2})$}
				\UnaryInfC{$\Gamma \vdash  y = e \cdot y$}

				\AxiomC{}
				\RightLabel{$(=I)$}
				\UnaryInfC{$\Gamma \vdash y = y$}

				\RightLabel{$(=E)$}
				\BinaryInfC{$\Gamma \vdash y = e \cdot y$}
			\end{prooftree}
			\item ~
			Let $\Gamma$ denote $M, (x \cdot y = e) \land (y \cdot x = e) \land (x \cdot z = e) \land (z \cdot x = e)$.
			\begin{prooftree}
				\AxiomC{}
				\RightLabel{$(Ax)$}
				\UnaryInfC{$\Gamma \vdash \forall a ((a \cdot e = a) \land (e \cdot a = a))$}
				\RightLabel{$(\forall E)$}
				\UnaryInfC{$\Gamma \vdash (y \cdot e = y) \land (e \cdot y = y)$}
				\RightLabel{$(\land E_{1})$}
				\UnaryInfC{$\Gamma \vdash y \cdot e = y$}

				\AxiomC{}
				\RightLabel{$(Ax)$}
				\RightLabel{$(\forall E)$}
				\UnaryInfC{$\Gamma \vdash \forall a \forall b \forall c((a \cdot b = e) \land (b \cdot a = e) \land (a \cdot c = e) \land (c \cdot a = e))$}
				\RightLabel{$(\forall E)$}
				\UnaryInfC{$\Gamma \vdash \forall b \forall c((x \cdot b = e) \land (b \cdot x = e) \land (x \cdot c = e) \land (c \cdot x = e))$}
				\RightLabel{$(\forall E)$}
				\UnaryInfC{$\Gamma \vdash \forall c((x \cdot y = e) \land (y \cdot x = e) \land (x \cdot c = e) \land (c \cdot x = e))$}
				\RightLabel{$(\forall E)$}
				\UnaryInfC{$\Gamma \vdash (x \cdot y = e) \land (y \cdot x = e) \land (x \cdot z = e) \land (z \cdot x = e)$}
				\RightLabel{$(\land E_{2})$}
				\UnaryInfC{$\Gamma \vdash (y \cdot x = e) \land (x \cdot z = e) \land (z \cdot x = e)$}
				\RightLabel{$(\land E_{2})$}
				\UnaryInfC{$\Gamma \vdash (x \cdot z = e) \land (z \cdot x = e)$}
				\RightLabel{$(\land E_{1})$}
				\UnaryInfC{$\Gamma \vdash x \cdot z = e$}

				\AxiomC{$\alpha$}

				\RightLabel{$(=E)$}
				\BinaryInfC{$\Gamma \vdash y \cdot e = z$}

				\RightLabel{$(=E)$}
				\BinaryInfC{$\Gamma \vdash y = z$}
				\RightLabel{$(\to I)$}	
				\UnaryInfC{$M \vdash ((x \cdot y = e) \land (y \cdot x = e) \land (x \cdot z = e) \land (z \cdot x = e)) \to y = z$}
				\RightLabel{$(\forall I)$}				
				\UnaryInfC{$M \vdash \forall c(((x \cdot y = e) \land (y \cdot x = e) \land (x \cdot c = e) \land (c \cdot x = e)) \to y = c)$}
				\RightLabel{$(\forall I)$}
				\UnaryInfC{$M \vdash \forall b \forall c(((x \cdot b = e) \land (b \cdot x = e) \land (x \cdot c = e) \land (c \cdot x = e)) \to b = c)$}
				\RightLabel{$(\forall I)$}
				\UnaryInfC{$M \vdash \forall a \forall b \forall c(((a \cdot b = e) \land (b \cdot a = e) \land (a \cdot c = e) \land (c \cdot a = e)) \to b = c)$}
			\end{prooftree}
			where $\alpha$ is the following tree :
			\begin{prooftree}
				\AxiomC{}
				\RightLabel{$(Ax)$}
				\UnaryInfC{$\Gamma \vdash \forall a \forall b \forall c ((b \cdot a) \cdot c = b \cdot (a \cdot c))$}
				\RightLabel{$(\forall E)$}
				\UnaryInfC{$\Gamma \vdash \forall b \forall c ((b \cdot x) \cdot c = b \cdot (x \cdot c))$}
				\RightLabel{$(\forall E)$}
				\UnaryInfC{$\Gamma \vdash \forall c ((y \cdot x) \cdot c = y \cdot (x \cdot c))$}
				\RightLabel{$(\forall E)$}
				\UnaryInfC{$\Gamma \vdash (y \cdot x) \cdot z = y \cdot (x \cdot z)$}

				\AxiomC{}
				\RightLabel{$(Ax)$}
				\UnaryInfC{$\Gamma \vdash \forall a \forall b \forall c ((a \cdot b = e) \land (b \cdot a = e) \land (a \cdot c = e) \land (c \cdot a = e))$}
				\RightLabel{$(\forall E)$}
				\UnaryInfC{$\Gamma \vdash \forall b \forall c ((x \cdot b = e) \land (b \cdot x = e) \land (x \cdot c = e) \land (c \cdot x = e))$}
				\RightLabel{$(\forall E)$}
				\UnaryInfC{$\Gamma \vdash \forall c ((x \cdot y = e) \land (y \cdot x = e) \land (x \cdot c = e) \land (c \cdot x = e))$}
				\RightLabel{$(\forall E)$}
				\UnaryInfC{$\Gamma \vdash (x \cdot y = e) \land (y \cdot x = e) \land (x \cdot z = e) \land (z \cdot x = e)$}
				\RightLabel{$(\land E_{2})$}
				\UnaryInfC{$\Gamma \vdash (y \cdot x = e) \land (x \cdot z = e) \land (z \cdot x = e)$}
				\RightLabel{$(\land E_{1})$}
				\UnaryInfC{$\Gamma \vdash e = y \cdot x$}

				\AxiomC{$\beta$}

				\RightLabel{$(=E)$}
				\BinaryInfC{$\Gamma \vdash (y \cdot x) \cdot z = z$}

				\RightLabel{$(=E)$}
				\BinaryInfC{$\Gamma \vdash y \cdot (x \cdot z) = z$}
			\end{prooftree}
			$\beta$ :
			\begin{prooftree}
				\AxiomC{}
				\RightLabel{$(Ax)$}
				\UnaryInfC{$\Gamma \vdash \forall a ((a \cdot e = a) \land (e \cdot a = a))$}
				\RightLabel{$(\forall E)$}
				\UnaryInfC{$\Gamma \vdash (z \cdot e = z) \land (e \cdot z = z)$}
				\RightLabel{$(\land E_{2})$}
				\UnaryInfC{$\Gamma \vdash z = e \cdot z$}
				
				\AxiomC{}
				\RightLabel{$(=I)$}
				\UnaryInfC{$\Gamma \vdash z = z$}

				\RightLabel{$(=E)$}
				\BinaryInfC{$\Gamma \vdash e \cdot z = z$}
			\end{prooftree}
		\end{enumerate}
	\end{enumerate}
\end{document}